parse_recursive_eq_gen

src/lowparse/LowParse.Spec.Recursive.fsti
@@ -99,6 +99,47 @@ let parse_recursive_eq'
 = parse_recursive_eq p b;
   tot_parse_synth_eq (parse_recursive_alt p (parse_recursive p)) p.synth_ b
 
+let spec_parse_recursive_payload
+  (p: parse_recursive_param)
+  (ih: parser (parse_recursive_kind p.parse_header_kind) p.t)
+  (h: p.header)
+: Tot (parser parse_recursive_payload_kind (parse_recursive_payload_t p.t p.header p.count h))
+= weaken parse_recursive_payload_kind (parse_nlist (p.count h) ih)
+
+let spec_parse_recursive_aux
+  (p: parse_recursive_param)
+  (#k: parser_kind)
+  (ph: parser k p.header)
+  (ih: parser (parse_recursive_kind p.parse_header_kind) p.t)
+: Tot (parser _ p.t)
+= (ph `parse_dtuple2` spec_parse_recursive_payload p ih) `parse_synth` p.synth_
+
+let parse_recursive_eq_gen
+  (p: parse_recursive_param)
+  (k: parser_kind)
+  (ph: parser k p.header)
+: Lemma
+  (requires (forall b . parse ph b == parse p.parse_header b))
+  (ensures (forall b. parse (parse_recursive p) b == parse (spec_parse_recursive_aux p ph (parser_of_tot_parser (parse_recursive p))) b))
+= let prf
+    (b: bytes)
+  : Lemma (parse (parse_recursive p) b == parse (spec_parse_recursive_aux p ph (parser_of_tot_parser (parse_recursive p))) b)
+  = let ih = (parser_of_tot_parser (parse_recursive p)) in
+    parse_recursive_eq' p b;
+    parse_synth_eq
+      (parse_dtuple2 ph (spec_parse_recursive_payload p ih))
+      p.synth_
+      b;
+    parse_dtuple2_eq ph (spec_parse_recursive_payload p ih) b;
+    match parse ph b with
+    | None -> ()
+    | Some (h, lenh) ->
+      let b' = Seq.slice b lenh (Seq.length b) in
+      tot_parse_nlist_parse_nlist (p.count h) (parse_recursive p) b';
+      ()
+  in
+  Classical.forall_intro prf
+
 let tot_parse_nlist_sum
   (#k: parser_kind)
   (#t: Type)
